Tealeaves/Simplification/MBinddt.v
@@ -10,12 +10,23 @@ Import
   ContainerFunctor.Notations
   Subset.Notations.
 
+(*|
+Miscellaneous
+|*)
+Ltac normalize_K :=
+  repeat
+    match goal with
+    | |- context[@K ?Ix] =>
+        unfold K, Ix
+    end.
+
 (** * Rewriting with binddt *)
 (******************************************************************************)
 Module ToBinddt.
 
-  Ltac rewrite_core_ops_to_binddt :=
+  Ltac rewrite_core_ops_to_mbinddt :=
     match goal with
+    (* map *)
     | |- context[mmap ?f ?t] =>
         ltac_trace "mmap_to_mbinddt";
         progress (rewrite mmap_to_mbinddt)
@@ -38,46 +49,12 @@ Module ToBinddt.
         progress (rewrite mbindt_to_mbinddt)
     end.
 
-  (*
-  Ltac rewrite_derived_ops_to_binddt T :=
-    match goal with
-    (* tolist *)
-    | |- context[tolist (F := T) ?t] =>
-        ltac_trace "tolist_to_binddt";
-        rewrite (tolist_to_binddt (T := T))
-    (* elements *)
-    | |- context[element_of (F := T) ?x ?t] =>
-        ltac_trace "element_of_to_binddt";
-        rewrite (element_of_to_binddt (T := T))
-    | |- context[element_ctx_of (T := T) (?n, ?l) ?t] =>
-        ltac_trace "element_ctx_of_to_binddt";
-        rewrite (element_ctx_of_to_binddt (T := T))
-    (* tosubset *)
-    | |- context[tosubset (F := T) ?t] =>
-        ltac_trace "tosubset_to_binddt";
-        rewrite (tosubset_to_binddt (T := T))
-    | |- context[toctxset (F := T) ?t] =>
-        ltac_trace "toctxset_to_binddt";
-        rewrite (toctxset_to_binddt (T := T))
-    (* foldMap *)
-    | |- context[foldMap (T := T) ?t] =>
-        ltac_trace "foldMap_to_binddt";
-        rewrite foldMap_to_traverse1, traverse_to_binddt
-    | |- context[foldMapd (T := T) ?t] =>
-        ltac_trace "foldMap_to_binddt";
-        rewrite (foldMapd_to_mapdt1 (T := T)),
-          (mapdt_to_binddt (T := T))
-    (* quantifiers *)
-    | |- context[Forall_ctx (T := T)  ?P] =>
-        ltac_trace "Forall_to_foldMapd";
-        unfold Forall_ctx
-    end.
-    *)
-
 End ToBinddt.
 
+Ltac cbn_mbinddt_post_hook := idtac.
+
 (*|
-If we find some <<binddt f t>>, simplify it with cbn.
+mbinddt
 |*)
 Ltac cbn_mbinddt :=
   match goal with
@@ -87,9 +64,148 @@ Ltac cbn_mbinddt :=
       let e := constr:(mbinddt (W := W) (T := T) U F
                          (H := H) (H0 := H0) (H1 := H1)
                          f t) in
-      cbn_subterm e
-      (*
-      let e' := eval cbn in e in
-        progress (change e with e')
-       *)
+      (* cbn_subterm e *)
+  let e' := eval cbn -[btgd btg] in e in
+    progress (change e with e'); cbn_mbinddt_post_hook
+
   end.
+
+Ltac simplify_mbinddt :=
+  cbn_mbinddt.
+
+(*|
+mbindd
+|*)
+Ltac cbn_mbindd :=
+  match goal with
+  | |- context[mbindd (W := ?W) (T := ?T)
+                ?U ?f ?t] =>
+      let e := constr:(mbindd (W := W) (T := T) U f t) in
+      cbn_subterm e
+  end.
+
+Ltac simplify_mbindd :=
+  match goal with
+  | |- context[mbindd (W := ?W) (T := ?T)
+                ?U ?f ?t] =>
+      rewrite ?mbindd_to_mbinddt;
+      simplify_mbinddt;
+      rewrite <- ?mbindd_to_mbinddt;
+      repeat simplify_applicative_I
+  end.
+
+(*|
+mbind
+|*)
+Ltac cbn_mbind :=
+  match goal with
+  | |- context[mbind (W := ?W) (T := ?T)
+                ?U ?f ?t] =>
+      let e := constr:(mbind (W := W) (T := T) U f t) in
+      cbn_subterm e
+  end.
+
+Ltac simplify_mbind :=
+  match goal with
+  | |- context[mbind (W := ?W) (T := ?T)
+                ?U ?f ?t] =>
+      rewrite ?mbind_to_mbindd;
+      simplify_mbindd;
+      rewrite <- ?mbind_to_mbindd;
+      repeat simplify_applicative_I
+  end.
+
+(*|
+mmapdt
+|*)
+Ltac cbn_mmapdt :=
+  match goal with
+  | |- context[mmapdt (W := ?W) (T := ?T)
+                ?U ?F ?f ?t] =>
+      let e := constr:(mmapdt (W := W) (T := T) U F
+                         f t) in
+      cbn_subterm e
+  end.
+
+Ltac simplify_mmapdt :=
+  cbn_mmapdt.
+
+(*|
+mmap
+|*)
+(*
+Ltac cbn_mmap :=
+  match goal with
+  | |- context[mmap (W := ?W) (T := ?T)
+                ?U ?f ?t] =>
+      let e := constr:(mmap (W := W) (T := T) U f t) in
+      cbn_subterm e
+  end.
+
+Ltac simplify_mmap :=
+  match goal with
+  | |- context[mmap (W := ?W) (T := ?T)
+                ?U ?f ?t] =>
+      rewrite ?mmap_to_mmapd;
+      simplify_mmapd;
+      rewrite <- ?mmap_to_mmapd;
+      repeat simplify_applicative_I
+  end.
+*)
+
+
+
+
+
+(*
+(** * Miscellaneous lemmas *)
+(******************************************************************************)
+Lemma filterk_incr : forall (A : Type) (k : K) (l : list (list K2 * (K * A))) (inc : list K2),
+    filterk k (map (F := list) (incr inc) l) = map (F := list) (incr inc) (filterk k l).
+Proof.
+  intros. induction l.
+  - easy.
+  - destruct a as  [ctx [j a]].
+    rewrite map_list_cons.
+    change (incr inc (ctx, (j, a))) with (inc ++ ctx, (j, a)).
+    compare values k and j.
+    + do 2 rewrite filterk_cons_eq.
+      autorewrite with tea_list.
+      now rewrite IHl.
+    + rewrite filterk_cons_neq; auto.
+      rewrite filterk_cons_neq; auto.
+Qed.
+
+(** * Simplification support *)
+(******************************************************************************)
+Lemma mextract_preincr2 :
+  forall `{ix: Index} {W : Type} {op : Monoid_op W}
+    {A: Type} {B : K -> Type} (f: forall k, A -> B k) (w : W),
+    (f ◻ const (extract (W := prod W) (A := A))) ◻ const (incr w) =
+      (f ◻ const (extract (W := prod W))).
+Proof.
+  intros.
+  ext k. ext [w' a].
+  reflexivity.
+Qed.
+
+
+Ltac simplify :=
+  match goal with
+  | |- context[mbinddt typ ?f ?t] =>
+      first [ rewrite mbinddt_type_rw1
+            | rewrite mbinddt_type_rw2
+            | rewrite mbinddt_type_rw3
+            | rewrite mbinddt_type_rw4 ]
+  | |- context[mbinddt term ?f ?t] =>
+      first [ rewrite mbinddt_term_rw1
+            | rewrite mbinddt_term_rw2
+            | rewrite mbinddt_term_rw3
+            | rewrite mbinddt_term_rw4
+            | rewrite mbinddt_term_rw5 ]
+  (* new stuff *)
+  | |- context[(?f ◻ allK extract) ◻ allK (incr ?w)] =>
+      rewrite mextract_preincr2
+  end.
+ *)
+
