Tealeaves/Simplification/Tests/SystemF_Binddt.v
@@ -1,11 +1,22 @@
 From Tealeaves Require Export
   Examples.SystemF.Syntax
-  Simplification.Tests.Support.
+  Simplification.Tests.Support
+  Simplification.MBinddt.
+
+Ltac cbn_mbinddt_post_hook ::=
+  try match goal with
+  | |- context[bind_type ?G ?f ?τ] =>
+      change (bind_type G f τ) with (mbinddt typ G f τ)
+  | |- context[bind_term ?G ?f ?t] =>
+      change (bind_term G f t) with (mbinddt term G f t)
+  end.
 
 #[local] Generalizable Variables G.
 #[local] Arguments mbinddt {ix} {W}%type_scope {T} U%function_scope
   {MBind} {F}%function_scope {H H0 H1 A B} _ _.
 
+(** ** <<mbinddt>> *)
+(******************************************************************************)
 Section rw_mbinddt.
 
   Context
@@ -13,57 +24,268 @@ Section rw_mbinddt.
     `{Applicative G}
     (f : forall k, list K * A -> G (SystemF k B)).
 
+  Ltac test_mbinddt :=
+    intros;
+    cbn_mbinddt;
+    try normalize_K;
+    conclude.
+
   Lemma mbinddt_type_rw1 : forall c,
       mbinddt typ f (ty_c c) = pure (ty_c c).
   Proof.
-    intros.
-    simplify_binddt.
-    reflexivity. Qed.
+    test_mbinddt.
+  Qed.
 
   Lemma mbinddt_type_rw2 : forall (a : A),
-      mbinddt typ f (ty_v a) = f KType (nil, a).
-  Proof. reflexivity. Qed.
+      mbinddt typ f (ty_v a) = f ktyp (nil, a).
+  Proof.
+    test_mbinddt.
+  Qed.
 
   Lemma mbinddt_type_rw3 : forall (t1 t2 : typ A),
       mbinddt typ f (ty_ar t1 t2) =
         pure ty_ar <⋆> mbinddt typ f t1 <⋆> mbinddt typ f t2.
-  Proof. reflexivity. Qed.
+  Proof.
+    test_mbinddt.
+  Qed.
 
   Lemma mbinddt_type_rw4 : forall (body : typ A),
       mbinddt typ f (ty_univ body) =
-        pure ty_univ <⋆> mbinddt typ (f ◻ const (incr [KType])) body.
-  Proof. reflexivity. Qed.
+        pure ty_univ <⋆> mbinddt typ (f ◻ allK (incr [ktyp])) body.
+  Proof.
+    test_mbinddt.
+  Qed.
 
   Lemma mbinddt_term_rw1 : forall (a : A),
-      mbinddt term f (tm_var a) = f KTerm (nil, a).
-  Proof. reflexivity. Qed.
+      mbinddt term f (tm_var a) = f ktrm (nil, a).
+  Proof.
+    test_mbinddt.
+  Qed.
 
   Lemma mbinddt_term_rw2 : forall (τ : typ A) (t : term A),
       mbinddt term f (tm_abs τ t) =
-        pure tm_abs <⋆> (mbinddt typ f τ) <⋆>
-          (mbinddt term (f ◻ const (incr [KTerm])) t).
-  Proof. reflexivity. Qed.
+        pure tm_abs <⋆> mbinddt typ f τ <⋆>
+          mbinddt term (f ◻ allK (incr [ktrm])) t.
+  Proof.
+    test_mbinddt.
+  Qed.
 
   Lemma mbinddt_term_rw3 : forall (t1 t2 : term A),
       mbinddt term f (tm_app t1 t2) =
         pure tm_app <⋆> (mbinddt term f t1) <⋆> (mbinddt term f t2).
-  Proof. reflexivity. Qed.
+  Proof.
+    test_mbinddt.
+  Qed.
 
   Lemma mbinddt_term_rw4 : forall (t : term A),
       mbinddt term f (tm_tab t) =
-        pure tm_tab <⋆> (mbinddt term (fun k => f k ∘ incr [KType]) t).
-  Proof. reflexivity. Qed.
+        pure tm_tab <⋆> mbinddt term (f ◻ allK (incr [ktyp])) t.
+  Proof.
+    test_mbinddt.
+  Qed.
 
   Lemma mbinddt_term_rw5 : forall (t: term A) (τ : typ A),
       mbinddt term f (tm_tap t τ) =
-        pure tm_tap <⋆> (mbinddt term f t) <⋆> (mbinddt typ f τ).
-  Proof. reflexivity. Qed.
+        pure tm_tap <⋆> mbinddt term f t <⋆> mbinddt typ f τ.
+  Proof.
+    test_mbinddt.
+  Qed.
 
 End rw_mbinddt.
 
-#[export] Hint Rewrite @mbinddt_term_rw1 @mbinddt_term_rw2 @mbinddt_term_rw3 @mbinddt_term_rw4 @mbinddt_term_rw5 : sysf_rw.
-#[export] Hint Rewrite @mbinddt_type_rw1 @mbinddt_type_rw2 @mbinddt_type_rw3 @mbinddt_type_rw4 : sysf_rw.
+(** ** <<mbindd>> *)
+(******************************************************************************)
+Section rw_mbindd.
 
+  Context
+    (A B : Type)
+    (f : forall k, list K * A -> SystemF k B).
+
+  Ltac test_mbindd :=
+    intros;
+    simplify_mbindd;
+    try normalize_K;
+    conclude.
+
+  Lemma mbindd_type_rw1 : forall c,
+      mbindd typ f (ty_c c) = ty_c c.
+  Proof.
+    test_mbindd.
+  Qed.
+
+  Lemma mbindd_type_rw2 : forall (a : A),
+      mbindd typ f (ty_v a) = f ktyp (nil, a).
+  Proof.
+    test_mbindd.
+  Qed.
+
+  Lemma mbindd_type_rw3 : forall (t1 t2 : typ A),
+      mbindd typ f (ty_ar t1 t2) =
+        ty_ar (mbindd typ f t1) (mbindd typ f t2).
+  Proof.
+    test_mbindd.
+  Qed.
+
+  Lemma mbindd_type_rw4 : forall (body : typ A),
+      mbindd typ f (ty_univ body) =
+        ty_univ (mbindd typ (f ◻ allK (incr [ktyp])) body).
+  Proof.
+    test_mbindd.
+  Qed.
+
+  Lemma mbindd_term_rw1 : forall (a : A),
+      mbindd term f (tm_var a) = f ktrm (nil, a).
+  Proof.
+    test_mbindd.
+  Qed.
+
+  Lemma mbindd_term_rw2 : forall (τ : typ A) (t : term A),
+      mbindd term f (tm_abs τ t) =
+        tm_abs (mbindd typ f τ)
+          (mbindd term (f ◻ allK (incr [ktrm])) t).
+  Proof.
+    test_mbindd.
+  Qed.
+
+  Lemma mbindd_term_rw3 : forall (t1 t2 : term A),
+      mbindd term f (tm_app t1 t2) =
+        tm_app  (mbindd term f t1) (mbindd term f t2).
+  Proof.
+    test_mbindd.
+  Qed.
+
+  Lemma mbindd_term_rw4 : forall (t : term A),
+      mbindd term f (tm_tab t) =
+        tm_tab (mbindd term (f ◻ allK (incr [ktyp])) t).
+  Proof.
+    test_mbindd.
+  Qed.
+
+  Lemma mbindd_term_rw5 : forall (t: term A) (τ : typ A),
+      mbindd term f (tm_tap t τ) =
+        tm_tap (mbindd term f t) (mbindd typ f τ).
+  Proof.
+    test_mbindd.
+  Qed.
+
+End rw_mbindd.
+
+(** ** <<kbindd>> *)
+(******************************************************************************)
+Section rw_kbindd.
+
+  Lemma kbindd_to_mbindd `{Ix:Index}: forall A (k: K) (f: list K * A -> SystemF k A),
+    kbindd typ k f = mbindd typ (btgd k f).
+  Proof.
+    reflexivity.
+  Qed.
+
+  Context
+    (A : Type)
+    (k : K2)
+    (f : list K2 * A -> SystemF k A).
+
+  Lemma btgd_compose_incr:
+    btgd k f ◻ allK (incr [ktyp]) =
+      btgd k (f ⦿ [ktyp]).
+  Proof.
+    intros.
+    ext j.
+    unfold allK, const.
+    unfold vec_compose.
+    compare values k and j.
+    { autorewrite with tea_tgt_eq.
+      reflexivity. }
+    { autorewrite with tea_tgt_neq.
+      reassociate -> on left.
+      rewrite extract_incr.
+      reflexivity. }
+  Qed.
+
+  Ltac simplify_kbindd :=
+    rewrite ?kbindd_to_mbindd;
+    simplify_mbindd;
+    rewrite <- ?kbindd_to_mbindd;
+    autorewrite* with tea_tgt;
+    try normalize_K.
+
+  Ltac test_kbindd :=
+    intros;
+    simplify_kbindd.
+
+  Lemma kbindd_type_rw1 : forall c,
+      kbindd typ k f (ty_c c) = ty_c c.
+  Proof.
+    test_kbindd.
+    conclude.
+  Qed.
+
+  Lemma kbindd_type_rw2 : forall (a : A),
+      kbindd typ k f (ty_v a) =
+        btgd k f ktyp ([], a).
+  Proof.
+    test_kbindd.
+    conclude.
+  Qed.
+
+  Lemma kbindd_type_rw3 : forall (t1 t2 : typ A),
+      kbindd typ k f (ty_ar t1 t2) =
+        ty_ar (kbindd typ k f t1) (kbindd typ k f t2).
+  Proof.
+    test_kbindd.
+    conclude.
+  Qed.
+
+  Lemma kbindd_type_rw4 : forall (body : typ A),
+      kbindd typ k f (ty_univ body) =
+        ty_univ (kbindd typ k (f ⦿ [ktyp]) body).
+  Proof.
+    intros.
+    simplify_kbindd.
+    setoid_rewrite btgd_compose_incr.
+    rewrite <- kbindd_to_mbindd.
+    normalize_K.
+    conclude.
+  Qed.
+
+  (*
+  Lemma kbindd_term_rw1 : forall (a : A),
+      kbindd term ktrm f (tm_var a) = f ktrm (nil, a).
+  Proof.
+    test_kbindd.
+  Qed.
+
+  Lemma kbindd_term_rw2 : forall (τ : typ A) (t : term A),
+      kbindd term k f (tm_abs τ t) =
+        tm_abs (kbindd typ k f τ)
+          (kbindd term k (f ◻ allK (incr [ktrm])) t).
+  Proof.
+    test_kbindd.
+  Qed.
+
+  Lemma kbindd_term_rw3 : forall (t1 t2 : term A),
+      kbindd term f (tm_app t1 t2) =
+        tm_app  (kbindd term f t1)  (kbindd term f t2).
+  Proof.
+    test_kbindd.
+  Qed.
+
+  Lemma kbindd_term_rw4 : forall (t : term A),
+      kbindd term f (tm_tab t) =
+        tm_tab (kbindd term (f ◻ allK (incr [ktyp])) t).
+  Proof.
+    test_kbindd.
+  Qed.
+
+  Lemma kbindd_term_rw5 : forall (t: term A) (τ : typ A),
+      kbindd term f (tm_tap t τ) =
+        tm_tap (kbindd term f t) (kbindd typ f τ).
+  Proof.
+    test_kbindd.
+  Qed.
+  *)
+
+End rw_kbindd.
 
 (*
 (** * Rewriting operations on <<typ>> *)
@@ -90,8 +312,8 @@ Section rw_mmapdt_type.
     reflexivity.
   Qed.
 
-  (* Why is this expressed with <⋆>? *)
-  Lemma rw_mmapdt_type2: forall (a: A), mmapdt typ F f (ty_v a) = pure ty_v <⋆> f KType (nil, a).
+  (* Why is this expressed with ? *)
+  Lemma rw_mmapdt_type2: forall (a: A), mmapdt typ F f (ty_v a) = pure ty_v  f ktyp (nil, a).
   Proof.
     intros.
     rewrite mmapdt_to_mbinddt.
@@ -102,7 +324,7 @@ Section rw_mmapdt_type.
 
   Lemma rw_mmapdt_type3: forall (t1 t2: typ A),
       mmapdt typ F f (ty_ar t1 t2) =
-        pure (ty_ar) <⋆> mmapdt typ F f t1 <⋆> mmapdt typ F f t2.
+        pure (ty_ar)  mmapdt typ F f t1  mmapdt typ F f t2.
   Proof.
     intros.
     rewrite mmapdt_to_mbinddt.
@@ -112,7 +334,7 @@ Section rw_mmapdt_type.
 
   Lemma rw_mmapdt_type4: forall (body: typ A),
       mmapdt typ F f (ty_univ body) =
-        pure (ty_univ) <⋆> mmapdt typ F (fun k => f k ∘ incr [KType]) body.
+        pure (ty_univ)  mmapdt typ F (fun k => f k ∘ incr [ktyp]) body.
   Proof.
     reflexivity.
   Qed.
@@ -134,13 +356,13 @@ Section rw_mbindd_type.
   Lemma rw_mbindd_type1: forall c, mbindd typ f (ty_c c) = ty_c c.
   Proof. reflexivity. Qed.
 
-  Lemma rw_mbindd_type2: forall (a: A), mbindd typ f (ty_v a) = f KType (nil, a).
+  Lemma rw_mbindd_type2: forall (a: A), mbindd typ f (ty_v a) = f ktyp (nil, a).
   Proof. reflexivity. Qed.
 
   Lemma rw_mbindd_type3: forall (t1 t2: typ A), mbindd typ f (ty_ar t1 t2) = ty_ar (mbindd typ f t1) (mbindd typ f t2).
   Proof. reflexivity. Qed.
 
-  Lemma rw_mbindd_type4: forall (body: typ A), mbindd typ f (ty_univ body) = ty_univ (mbindd typ (fun k => f k ∘ incr [KType]) body).
+  Lemma rw_mbindd_type4: forall (body: typ A), mbindd typ f (ty_univ body) = ty_univ (mbindd typ (fun k => f k ∘ incr [ktyp]) body).
   Proof. reflexivity. Qed.
 
 End rw_mbindd_type.
@@ -158,7 +380,7 @@ Section rw_mbind_type.
   Lemma rw_mbind_type1: forall c, mbind typ f (ty_c c) = ty_c c.
   Proof. reflexivity. Qed.
 
-  Lemma rw_mbind_type2: forall (a: A), mbind typ f (ty_v a) = f KType a.
+  Lemma rw_mbind_type2: forall (a: A), mbind typ f (ty_v a) = f ktyp a.
   Proof. reflexivity. Qed.
 
   Lemma rw_mbind_type3: forall (t1 t2: typ A), mbind typ f (ty_ar t1 t2) = ty_ar (mbind typ f t1) (mbind typ f t2).
@@ -173,7 +395,7 @@ End rw_mbind_type.
 
 #[export] Hint Rewrite @rw_mbind_type1 @rw_mbind_type2 @rw_mbind_type3 @rw_mbind_type4: sysf_rw.
 
-(** *** <<kbindd>> with <<KType>> *)
+(** *** <<kbindd>> with <<ktyp>> *)
 (******************************************************************************)
 Section rw_kbindd_type.
 
@@ -181,16 +403,16 @@ Section rw_kbindd_type.
     (A: Type)
     (f: list K * A -> typ A).
 
-  Lemma rw_kbindd_KType_type1: forall c, kbindd typ KType f (ty_c c) = ty_c c.
+  Lemma rw_kbindd_ktyp_type1: forall c, kbindd typ ktyp f (ty_c c) = ty_c c.
   Proof. reflexivity. Qed.
 
-  Lemma rw_kbindd_KType_type2: forall a, kbindd typ KType f (ty_v a) = f (nil, a).
+  Lemma rw_kbindd_ktyp_type2: forall a, kbindd typ ktyp f (ty_v a) = f (nil, a).
   Proof. reflexivity. Qed.
 
-  Lemma rw_kbindd_KType_type3: forall (t1 t2: typ A), kbindd typ KType f (ty_ar t1 t2) = ty_ar (kbindd typ KType f t1) (kbindd typ KType f t2).
+  Lemma rw_kbindd_ktyp_type3: forall (t1 t2: typ A), kbindd typ ktyp f (ty_ar t1 t2) = ty_ar (kbindd typ ktyp f t1) (kbindd typ ktyp f t2).
   Proof. reflexivity. Qed.
 
-  Lemma rw_kbindd_KType_type4: forall (body: typ A), kbindd typ KType f (ty_univ body) = ty_univ (kbindd typ KType (f ∘ incr [KType]) body).
+  Lemma rw_kbindd_ktyp_type4: forall (body: typ A), kbindd typ ktyp f (ty_univ body) = ty_univ (kbindd typ ktyp (f ∘ incr [ktyp]) body).
   Proof.
     intros. unfold kbindd. simpl_F.
     do 2 fequal. now ext j [w a].
@@ -198,9 +420,9 @@ Section rw_kbindd_type.
 
 End rw_kbindd_type.
 
-#[export] Hint Rewrite @rw_kbindd_KType_type1 @rw_kbindd_KType_type2 @rw_kbindd_KType_type3 @rw_kbindd_KType_type4: sysf_rw.
+#[export] Hint Rewrite @rw_kbindd_ktyp_type1 @rw_kbindd_ktyp_type2 @rw_kbindd_ktyp_type3 @rw_kbindd_ktyp_type4: sysf_rw.
 
-(** *** <<kbindd>> with <<KTerm>> *)
+(** *** <<kbindd>> with <<ktrm>> *)
 (******************************************************************************)
 Section rw_kbindd_type.
 
@@ -208,16 +430,16 @@ Section rw_kbindd_type.
     (A: Type)
     (f: list K * A -> term A).
 
-  Lemma rw_kbindd_KTerm_type1: forall c, kbindd typ KTerm f (ty_c c) = ty_c c.
+  Lemma rw_kbindd_ktrm_type1: forall c, kbindd typ ktrm f (ty_c c) = ty_c c.
   Proof. reflexivity. Qed.
 
-  Lemma rw_kbindd_KTerm_type2: forall a, kbindd typ KTerm f (ty_v a) = ty_v a.
+  Lemma rw_kbindd_ktrm_type2: forall a, kbindd typ ktrm f (ty_v a) = ty_v a.
   Proof. reflexivity. Qed.
 
-  Lemma rw_kbindd_KTerm_type3: forall (t1 t2: typ A), kbindd typ KTerm f (ty_ar t1 t2) = ty_ar (kbindd typ KTerm f t1) (kbindd typ KTerm f t2).
+  Lemma rw_kbindd_ktrm_type3: forall (t1 t2: typ A), kbindd typ ktrm f (ty_ar t1 t2) = ty_ar (kbindd typ ktrm f t1) (kbindd typ ktrm f t2).
   Proof. reflexivity. Qed.
 
-  Lemma rw_kbindd_KTerm_type4: forall (body: typ A), kbindd typ KTerm f (ty_univ body) = ty_univ (kbindd typ KTerm (f ∘ incr [KType]) body).
+  Lemma rw_kbindd_ktrm_type4: forall (body: typ A), kbindd typ ktrm f (ty_univ body) = ty_univ (kbindd typ ktrm (f ∘ incr [ktyp]) body).
   Proof.
     intros. unfold kbindd. simpl_F.
     do 2 fequal. now ext j [w a].
@@ -225,9 +447,9 @@ Section rw_kbindd_type.
 
 End rw_kbindd_type.
 
-#[export] Hint Rewrite @rw_kbindd_KTerm_type1 @rw_kbindd_KTerm_type2 @rw_kbindd_KTerm_type3 @rw_kbindd_KTerm_type4: sysf_rw.
+#[export] Hint Rewrite @rw_kbindd_ktrm_type1 @rw_kbindd_ktrm_type2 @rw_kbindd_ktrm_type3 @rw_kbindd_ktrm_type4: sysf_rw.
 
-(** *** <<kbind>> with <<KType>> *)
+(** *** <<kbind>> with <<ktyp>> *)
 (******************************************************************************)
 Section rw_kbind_type.
 
@@ -235,25 +457,25 @@ Section rw_kbind_type.
     (A: Type)
     (f: A -> typ A).
 
-  Lemma rw_kbind_KType_type1: forall c, kbind typ KType f (ty_c c) = ty_c c.
+  Lemma rw_kbind_ktyp_type1: forall c, kbind typ ktyp f (ty_c c) = ty_c c.
   Proof. reflexivity. Qed.
 
-  Lemma rw_kbind_KType_type2: forall a, kbind typ KType f (ty_v a) = f a.
+  Lemma rw_kbind_ktyp_type2: forall a, kbind typ ktyp f (ty_v a) = f a.
   Proof. reflexivity. Qed.
 
-  Lemma rw_kbind_KType_type3: forall (t1 t2: typ A), kbind typ KType f (ty_ar t1 t2) = ty_ar (kbind typ KType f t1) (kbind typ KType f t2).
+  Lemma rw_kbind_ktyp_type3: forall (t1 t2: typ A), kbind typ ktyp f (ty_ar t1 t2) = ty_ar (kbind typ ktyp f t1) (kbind typ ktyp f t2).
   Proof. reflexivity. Qed.
 
-  Lemma rw_kbind_KType_type4: forall (body: typ A), kbind typ KType f (ty_univ body) = ty_univ (kbind typ KType f body).
+  Lemma rw_kbind_ktyp_type4: forall (body: typ A), kbind typ ktyp f (ty_univ body) = ty_univ (kbind typ ktyp f body).
   Proof.
     intros. unfold kbind. now simpl_F.
   Qed.
 
 End rw_kbind_type.
 
-#[export] Hint Rewrite @rw_kbind_KType_type1 @rw_kbind_KType_type2 @rw_kbind_KType_type3 @rw_kbind_KType_type4: sysf_rw.
+#[export] Hint Rewrite @rw_kbind_ktyp_type1 @rw_kbind_ktyp_type2 @rw_kbind_ktyp_type3 @rw_kbind_ktyp_type4: sysf_rw.
 
-(** *** <<kbind>> with <<KTerm>> *)
+(** *** <<kbind>> with <<ktrm>> *)
 (******************************************************************************)
 Section rw_kbind_type.
 
@@ -261,22 +483,22 @@ Section rw_kbind_type.
     (A: Type)
     (f: A -> term A).
 
-  Lemma rw_kbind_KTerm_type1: forall c, kbind typ KTerm f (ty_c c) = ty_c c.
+  Lemma rw_kbind_ktrm_type1: forall c, kbind typ ktrm f (ty_c c) = ty_c c.
   Proof. reflexivity. Qed.
 
-  Lemma rw_kbind_KTerm_type2: forall a, kbind typ KTerm f (ty_v a) = ty_v a.
+  Lemma rw_kbind_ktrm_type2: forall a, kbind typ ktrm f (ty_v a) = ty_v a.
   Proof. reflexivity. Qed.
 
-  Lemma rw_kbind_KTerm_type3: forall (t1 t2: typ A), kbind typ KTerm f (ty_ar t1 t2) = ty_ar (kbind typ KTerm f t1) (kbind typ KTerm f t2).
+  Lemma rw_kbind_ktrm_type3: forall (t1 t2: typ A), kbind typ ktrm f (ty_ar t1 t2) = ty_ar (kbind typ ktrm f t1) (kbind typ ktrm f t2).
   Proof. reflexivity. Qed.
 
-  Lemma rw_kbind_KTerm_type4: forall (body: typ A), kbind typ KTerm f (ty_univ body) = ty_univ (kbind typ KTerm f body).
+  Lemma rw_kbind_ktrm_type4: forall (body: typ A), kbind typ ktrm f (ty_univ body) = ty_univ (kbind typ ktrm f body).
   Proof.
     intros. unfold kbind. now simpl_F.
   Qed.
 
 End rw_kbind_type.
 
-#[export] Hint Rewrite @rw_kbind_KTerm_type1 @rw_kbind_KTerm_type2 @rw_kbind_KTerm_type3 @rw_kbind_KTerm_type4: sysf_rw.
+#[export] Hint Rewrite @rw_kbind_ktrm_type1 @rw_kbind_ktrm_type2 @rw_kbind_ktrm_type3 @rw_kbind_ktrm_type4: sysf_rw.
 
 *)
